examples/linked-lists/rev_why.v
@@ -3,127 +3,154 @@ Require Why.
 
 Require LinkedLists.
 
-(* Why obligation from file "rev.mlw", characters 1212-1684 *)
+(* Why obligation from file "rev.mlw", characters 1173-1631 *)
 Lemma rev_po_1 : 
   (p0: pointer)
   (Ltl: pointer_store)
-  (Pre4: (EX l:plist | (list_of Ltl p0 l)))
-  (result: pointer)
-  (Post8: result = p0)
-  (result0: pointer)
-  (Post7: result0 = result)
-  (p1: pointer)
-  (Post1: p1 = null)
-  (well_founded tl_order).
+  (Pre4: (is_list Ltl p0))
+  (p: pointer)
+  (Post8: p = p0)
+  (r: pointer)
+  (Post7: r = p)
+  (p2: pointer)
+  (Post1: p2 = null)
+  (well_founded ll_order).
 Proof.
-Intros; Exact tl_order_wf.
+Auto.
 Save.
 
-(* Why obligation from file "rev.mlw", characters 1567-1675 *)
+Lemma disjoint_cons : 
+  (l1,l2:plist)(x:pointer)
+  (disjoint l1 (cons x l2)) -> 
+  ~(In x l2) ->
+  (disjoint (cons x l1) l2).
+Proof.
+Unfold disjoint; Intuition.
+Elim (in_inv H); Intuition.
+Subst x; Intuition.
+Apply H1 with x0; Intuition.
+Elim (in_inv H3); Intuition.
+Subst x; Intuition.
+Apply H1 with x0; Intuition.
+Save.
+
+Lemma app_rev_cons : 
+  (A:Set)(l1,l2:(list A))(x:A)
+  (app (rev l1) (cons x l2)) = (app (rev (cons x l1)) l2).
+Proof.
+Intros; Simpl.
+Rewrite app_ass; Auto.
+Save.
+
+
+(* Why obligation from file "rev.mlw", characters 1534-1622 *)
 Lemma rev_po_2 : 
   (p0: pointer)
-  (Lhd: int_store)
   (Ltl: pointer_store)
-  (Pre4: (EX l:plist | (list_of Ltl p0 l)))
-  (result: pointer)
-  (Post8: result = p0)
-  (result0: pointer)
-  (Post7: result0 = result)
-  (p1: pointer)
-  (Post1: p1 = null)
-  (Variant1: Triple)
-  (Ltl0: pointer_store)
+  (Pre4: (is_list Ltl p0))
+  (p: pointer)
+  (Post8: p = p0)
+  (r: pointer)
+  (Post7: r = p)
   (p2: pointer)
-  (r0: pointer)
-  (Pre3: Variant1 = (triple Lhd Ltl0 r0))
-  (Pre2: (EX lp:plist |
-          (EX lr:plist | (list_of Ltl0 p2 lp) /\ (list_of Ltl0 r0 lr) /\
-           (disjoint lp lr) /\
-           ((l:plist) ((list_of Ltl0 p0 l) -> (app (rev lr) lp) = (rev l))))))
-  (Test2: ~(r0 = null))
-  (result3: pointer)
-  (Post5: result3 = r0)
-  (r1: pointer)
-  (Post2: r1 = (access_pointer Ltl0 r0))
-  (Ltl1: pointer_store)
-  (Post3: Ltl1 = (update_pointer Ltl0 result3 p2))
+  (Post1: p2 = null)
+  (Variant1: StorePointerPair)
+  (Ltl0: pointer_store)
   (p3: pointer)
-  (Post4: p3 = result3)
+  (r1: pointer)
+  (Pre3: Variant1 = (store_pointer_pair Ltl0 r1))
+  (Pre2: (EX lp:plist |
+          (EX lr:plist | (llist Ltl0 p3 lp) /\ (llist Ltl0 r1 lr) /\
+           (disjoint lp lr) /\
+           ((l:plist) ((llist Ltl p0 l) -> (app (rev lr) lp) = (rev l))))))
+  (Test2: ~(r1 = null))
+  (q: pointer)
+  (Post5: q = r1)
+  (r2: pointer)
+  (Post2: r2 = (pget Ltl0 r1))
+  (Ltl1: pointer_store)
+  (Post3: Ltl1 = (pset Ltl0 q p3))
+  (p4: pointer)
+  (Post4: p4 = q)
   (EX lp:plist |
-   (EX lr:plist | (list_of Ltl1 p3 lp) /\ (list_of Ltl1 r1 lr) /\
+   (EX lr:plist | (llist Ltl1 p4 lp) /\ (llist Ltl1 r2 lr) /\
     (disjoint lp lr) /\
-    ((l:plist) ((list_of Ltl1 p0 l) -> (app (rev lr) lp) = (rev l))))) /\
-  (tl_order (triple Lhd Ltl1 r1) (triple Lhd Ltl0 r0)).
+    ((l:plist) ((llist Ltl p0 l) -> (app (rev lr) lp) = (rev l))))) /\
+  (ll_order (store_pointer_pair Ltl1 r2) (store_pointer_pair Ltl0 r1)).
 Proof.
 Intuition.
 Elim Pre2; Clear Pre2; Intuition.
 Elim H; Clear H; Intuition.
 Subst.
 Inversion H.
-Absurd r0=null; Intuition.
-Exists (cons r0 x); Exists l; Subst; Intuition.
-Apply List_of_cons; Intuition.
-Unfold access_pointer; Unfold 2 update_pointer.
-Rewrite pupdate_paccess_same; Auto.
-Apply list_of_update_same; Auto.
+Absurd r1=null; Intuition.
+Exists (cons r1 x); Exists l; Subst; Intuition.
+Unfold llist; Apply Path_cons; Intuition.
+Rewrite PointerStore.get_set_same; Auto.
+Apply llist_pset_same; Auto.
 Unfold disjoint in H1; Intuition.
-Apply (H7 r0); Auto.
+Apply (H7 r1); Auto.
 Rewrite <- H6; Auto with *.
-Apply list_of_update_same; Auto.
-
+Apply llist_pset_same; Auto.
+Apply llist_not_starting with Ltl0; Auto.
+Apply disjoint_cons.
+Rewrite H6; Auto.
+Apply llist_not_starting with Ltl0; Auto.
+Rewrite app_rev_cons.
+Rewrite H6; Apply H3; Auto.
+Unfold ll_order store_pointer_pair.
 
 Save.
 
-(* Why obligation from file "rev.mlw", characters 1212-1684 *)
+(* Why obligation from file "rev.mlw", characters 1173-1631 *)
 Lemma rev_po_3 : 
   (p0: pointer)
-  (Lhd: int_store)
   (Ltl: pointer_store)
-  (Pre4: (EX l:plist | (list_of Ltl p0 l)))
-  (result: pointer)
-  (Post8: result = p0)
-  (result0: pointer)
-  (Post7: result0 = result)
-  (p1: pointer)
-  (Post1: p1 = null)
-  (Variant1: Triple)
-  (Ltl0: pointer_store)
+  (Pre4: (is_list Ltl p0))
+  (p: pointer)
+  (Post8: p = p0)
+  (r: pointer)
+  (Post7: r = p)
   (p2: pointer)
-  (r0: pointer)
-  (Pre3: Variant1 = (triple Lhd Ltl0 r0))
-  (Pre2: (EX lp:plist |
-          (EX lr:plist | (list_of Ltl0 p2 lp) /\ (list_of Ltl0 r0 lr) /\
-           (disjoint lp lr) /\
-           ((l:plist) ((list_of Ltl0 p0 l) -> (app (rev lr) lp) = (rev l))))))
-  (Test2: ~(r0 = null))
-  (Ltl1: pointer_store)
+  (Post1: p2 = null)
+  (Variant1: StorePointerPair)
+  (Ltl0: pointer_store)
   (p3: pointer)
   (r1: pointer)
+  (Pre3: Variant1 = (store_pointer_pair Ltl0 r1))
+  (Pre2: (EX lp:plist |
+          (EX lr:plist | (llist Ltl0 p3 lp) /\ (llist Ltl0 r1 lr) /\
+           (disjoint lp lr) /\
+           ((l:plist) ((llist Ltl p0 l) -> (app (rev lr) lp) = (rev l))))))
+  (Test2: ~(r1 = null))
+  (Ltl1: pointer_store)
+  (p4: pointer)
+  (r2: pointer)
   (Post9: (EX lp:plist |
-           (EX lr:plist | (list_of Ltl1 p3 lp) /\ (list_of Ltl1 r1 lr) /\
+           (EX lr:plist | (llist Ltl1 p4 lp) /\ (llist Ltl1 r2 lr) /\
             (disjoint lp lr) /\
-            ((l:plist) ((list_of Ltl1 p0 l) -> (app (rev lr) lp) = (rev l))))) /\
-          (tl_order (triple Lhd Ltl1 r1) (triple Lhd Ltl0 r0)))
-  (tl_order (triple Lhd Ltl1 r1) Variant1).
+            ((l:plist) ((llist Ltl p0 l) -> (app (rev lr) lp) = (rev l))))) /\
+          (ll_order (store_pointer_pair Ltl1 r2) (store_pointer_pair Ltl0 r1)))
+  (ll_order (store_pointer_pair Ltl1 r2) Variant1).
 Proof.
 Destruct result3; Intuition.
 Save.
 
-(* Why obligation from file "rev.mlw", characters 1261-1485 *)
+(* Why obligation from file "rev.mlw", characters 1222-1445 *)
 Lemma rev_po_4 : 
   (p0: pointer)
   (Ltl: pointer_store)
-  (Pre4: (EX l:plist | (list_of Ltl p0 l)))
-  (result: pointer)
-  (Post8: result = p0)
-  (result0: pointer)
-  (Post7: result0 = result)
-  (p1: pointer)
-  (Post1: p1 = null)
+  (Pre4: (is_list Ltl p0))
+  (p: pointer)
+  (Post8: p = p0)
+  (r: pointer)
+  (Post7: r = p)
+  (p2: pointer)
+  (Post1: p2 = null)
   (EX lp:plist |
-   (EX lr:plist | (list_of Ltl p1 lp) /\ (list_of Ltl result0 lr) /\
+   (EX lr:plist | (llist Ltl p2 lp) /\ (llist Ltl r lr) /\
     (disjoint lp lr) /\
-    ((l:plist) ((list_of Ltl p0 l) -> (app (rev lr) lp) = (rev l))))).
+    ((l:plist) ((llist Ltl p0 l) -> (app (rev lr) lp) = (rev l))))).
 Proof.
 Intuition; Discriminate H3 Orelse Clear H3.
 Subst.
@@ -150,27 +177,27 @@ Absurd p1=null; Auto.
 Save.
 
 
-(* Why obligation from file "rev.mlw", characters 1690-1692 *)
+(* Why obligation from file "rev.mlw", characters 1637-1639 *)
 Lemma rev_po_5 : 
   (p0: pointer)
   (Ltl: pointer_store)
-  (Pre4: (EX l:plist | (list_of Ltl p0 l)))
-  (result: pointer)
-  (Post8: result = p0)
-  (result0: pointer)
-  (Post7: result0 = result)
-  (p1: pointer)
-  (Post1: p1 = null)
-  (Ltl0: pointer_store)
+  (Pre4: (is_list Ltl p0))
+  (p: pointer)
+  (Post8: p = p0)
+  (r: pointer)
+  (Post7: r = p)
   (p2: pointer)
-  (r0: pointer)
+  (Post1: p2 = null)
+  (Ltl0: pointer_store)
+  (p3: pointer)
+  (r1: pointer)
   (Post6: (EX lp:plist |
-           (EX lr:plist | (list_of Ltl0 p2 lp) /\ (list_of Ltl0 r0 lr) /\
+           (EX lr:plist | (llist Ltl0 p3 lp) /\ (llist Ltl0 r1 lr) /\
             (disjoint lp lr) /\
-            ((l:plist) ((list_of Ltl0 p0 l) -> (app (rev lr) lp) = (rev l))))) /\
-          r0 = null)
-  (EX l:plist | (list_of Ltl0 p2 l) /\
-   ((l0:plist) ((list_of Ltl0 p0 l0) -> l = (rev l0)))).
+            ((l:plist) ((llist Ltl p0 l) -> (app (rev lr) lp) = (rev l))))) /\
+          r1 = null)
+  (EX l:plist | (llist Ltl0 p3 l) /\
+   ((l0:plist) ((llist Ltl0 p0 l0) -> l = (rev l0)))).
 Proof.
 (* FILL PROOF HERE *)
 Save.
